Prove monad identity laws

ProgTheorems.v
@@ -2,6 +2,8 @@ Require Import Automation.
 Require Import Prog.
 Require Import ProofIrrelevance.
 
+Set Implicit Arguments.
+
 (** Here we prove some basic sanity checks on prog and its semantics. *)
 
 Hint Constructors exec.
@@ -32,6 +34,61 @@ Proof.
   induction p; intros;
     inv_exec;
     eauto.
+Qed.
+
+(** These are the monad laws
+
+TODO: explain what the monad is and what these monad laws mean (specifically,
+we're proving that exec treats programs up to the monad laws as equivalences
+between programs).
+ *)
+
+Definition exec_equiv T (p p': prog3 T) :=
+  forall sigma r, exec p sigma r <-> exec p' sigma r.
+
+Lemma exec_ret : forall T (v:T) sigma r,
+    exec (Ret v) sigma r ->
+    match r with
+    | Finished v' sigma' => v = v' /\ sigma = sigma'
+    | Crashed sigma' => sigma = sigma'
+    | Failed => False
+    end.
+Proof.
+  intros.
+  inv_exec; simpl in *;
+    try match goal with
+        | [ H: StepTo _ _ = StepTo _ _ |- _ ] =>
+          inversion H; subst
+        end;
+    intuition; try congruence.
+Qed.
+
+Ltac cleanup_exec :=
+  match goal with
+  | [ H: step (Bind _ _) _ = _ |- _ ] =>
+    try solve [ simpl in H; inversion H ]
+  | [ H: exec (Ret _) _ ?r |- _ ] =>
+    first [ is_var r |
+            apply exec_ret in H; safe_intuition; subst;
+          try solve [ exfalso; apply H ] ]
+  end.
+
+Theorem monad_left_id : forall T T' (p: T' -> prog3 T) v,
+    exec_equiv (Bind (Ret v) p) (p v).
+Proof.
+  unfold exec_equiv; split; intros.
+  - inv_exec; try cleanup_exec; eauto.
+  - eapply ExecBindFinished; eauto.
+    eapply ExecStepTo; eauto.
+Qed.
+
+Theorem monad_right_id : forall T (p: prog3 T),
+    exec_equiv (Bind p (fun v => Ret v)) p.
+Proof.
+  unfold exec_equiv; split; intros.
+  - destruct r; inv_exec; try cleanup_exec; eauto.
+    eapply can_crash_at_end; eauto.
+  - destruct r; eauto.
 Qed.
 
 (* Local Variables: *)
